Improve big step semantics, such that step indexed semantics is an instance of it.

HoareLogic/BigStepSemantics.v
@@ -17,7 +17,6 @@ Definition lift_access
           (ms2: MetaState state): Prop :=
   lift_relation (fun s => access s c) ms1 ms2.
 
-
 Definition safe
            {P: ProgrammingLanguage}
            {state: Type}
@@ -39,3 +38,119 @@ Definition term_norm
 Class NormalBigStepSemantics (P: ProgrammingLanguage) (state: Type) (BSS: BigStepSemantics P state): Type := {
   access_defined: forall s c, exists ms, access s c ms
 }.
+
+Class SABigStepSemantics (P: ProgrammingLanguage) (state: Type) {J: Join state} {kiM: KripkeIntuitionisticModel state} (BSS: BigStepSemantics P state): Type := {
+  frame_property: forall m mf m' c n', join m mf m' -> access m' c n' -> exists n nf, Korder nf mf /\ lift_join n (Terminating nf) n' /\ access m c n
+}.
+
+Inductive loop_access_fin
+          {state: Type}
+          {kiM: KripkeIntuitionisticModel state}
+          (R: state -> MetaState state -> Prop)
+          (test: state -> Prop): state -> MetaState state -> Prop :=
+| loop_access_Terminating:
+    forall s1 s2,
+      ~ test s1 ->
+      Korder s2 s1 ->
+      loop_access_fin R test s1 (Terminating s2)
+| loop_access_Error:
+    forall s1 s2,
+      test s1 ->
+      Korder s2 s1 ->
+      R s2 Error ->
+      loop_access_fin R test s1 Error
+| loop_access_fin_NonTerminating:
+    forall s1 s2,
+      test s1 ->
+      Korder s2 s1 ->
+      R s2 NonTerminating ->
+      loop_access_fin R test s1 NonTerminating
+| loop_access_step:
+    forall s1 s2 s3 s4 ms,
+      test s1 ->
+      Korder s2 s1 ->
+      R s2 (Terminating s3) ->
+      Korder s4 s3 ->
+      loop_access_fin R test s4 ms ->
+      loop_access_fin R test s1 ms.
+
+Inductive loop_access_inf
+          {state: Type}
+          {kiM: KripkeIntuitionisticModel state}
+          (R: state -> MetaState state -> Prop)
+          (test: state -> Prop): state -> Prop :=
+| loop_access_inf_NonTerminating:
+    forall (s1 s2 s3: nat -> state),
+      (forall n, test (s1 n)) ->
+      (forall n, Korder (s2 n) (s1 n)) ->
+      (forall n, R (s2 n) (Terminating (s3 n))) ->
+      (forall n, Korder (s1 (S n)) (s3 n)) ->
+      loop_access_inf R test (s1 0).
+
+Inductive loop_access
+          {state: Type}
+          {kiM: KripkeIntuitionisticModel state}
+          (R: state -> MetaState state -> Prop)
+          (test: state -> Prop): state -> MetaState state -> Prop :=
+| loop_access_loop_access_fin:
+    forall s ms, loop_access_fin R test s ms ->
+      loop_access R test s ms
+| loop_access_loop_access_inf:
+    forall s, loop_access_inf R test s ->
+      loop_access R test s NonTerminating.
+
+Module Total.
+
+Class ImpBigStepSemantics (P: ProgrammingLanguage) {iP: ImperativeProgrammingLanguage P} (state: Type) {kiM: KripkeIntuitionisticModel state} (BSS: BigStepSemantics P state): Type := {
+  eval_bool: state -> bool_expr -> Prop;
+  eval_bool_stable: forall b, Korder_stable (fun s => eval_bool s b);
+  access_Ssequence: forall c1 c2 s ms,
+    access s (Ssequence c1 c2) ms ->
+    exists ms' ms'',
+      access s c1 ms' /\ lift_Korder ms'' ms' /\ lift_access ms'' c2 ms;
+  access_Sifthenelse: forall b c1 c2 s ms,
+    access s (Sifthenelse b c1 c2) ms ->
+    (eval_bool s b /\ exists s', Korder s' s /\ access s' c1 ms) \/
+    (~ eval_bool s b /\ exists s', Korder s' s /\ access s' c2 ms);
+  access_Swhile: forall b c s ms,
+    access s (Swhile b c) ms ->
+    loop_access (fun s ms => access s c ms) (fun s => eval_bool s b) s ms
+}.
+
+End Total.
+
+Module Partial.
+
+Class ImpBigStepSemantics (P: ProgrammingLanguage) {iP: ImperativeProgrammingLanguage P} (state: Type) {kiM: KripkeIntuitionisticModel state} (BSS: BigStepSemantics P state): Type := {
+  eval_bool: state -> bool_expr -> Prop;
+  eval_bool_stable: forall b, Korder_stable (fun s => eval_bool s b);
+  access_Ssequence: forall c1 c2 s ms,
+    access s (Ssequence c1 c2) ms ->
+    exists ms' ms'',
+      access s c1 ms' /\ lift_Korder ms'' ms' /\ lift_access ms'' c2 ms;
+  access_Sifthenelse: forall b c1 c2 s ms,
+    access s (Sifthenelse b c1 c2) ms ->
+    ms = NonTerminating \/
+    (eval_bool s b /\ exists s', Korder s' s /\ access s' c1 ms) \/
+    (~ eval_bool s b /\ exists s', Korder s' s /\ access s' c2 ms);
+  access_Swhile: forall b c s ms,
+    access s (Swhile b c) ms ->
+    ms = NonTerminating \/
+    loop_access_fin (fun s ms => access s c ms) (fun s => eval_bool s b) s ms
+}.
+
+End Partial.
+
+Instance Total2Partial_ImpBigStepSemantics {P: ProgrammingLanguage} {iP: ImperativeProgrammingLanguage P} (state: Type) {kiM: KripkeIntuitionisticModel state} {BSS: BigStepSemantics P state} (iBSS: Total.ImpBigStepSemantics P state BSS): Partial.ImpBigStepSemantics P state BSS.
+Proof.
+  refine (Partial.Build_ImpBigStepSemantics _ _ _ _ _ Total.eval_bool Total.eval_bool_stable _ _ _).
+  + apply Total.access_Ssequence.
+  + intros.
+    pose proof Total.access_Sifthenelse b c1 c2 s ms H.
+    tauto.
+  + intros.
+    pose proof Total.access_Swhile b c s ms H.
+    destruct H0; tauto.
+Defined.
+
+
