HoareLogic/Sound_Imp.v
@@ -17,81 +17,10 @@ Import SeparationLogicNotation.
 Import KripkeModelSingleNotation.
 Import KripkeModelNotation_Intuitionistic.
 
-Inductive loop_access_fin
-          {state: Type}
-          {kiM: KripkeIntuitionisticModel state}
-          (R: state -> MetaState state -> Prop)
-          (test: state -> Prop): state -> MetaState state -> Prop :=
-| loop_access_Terminating:
-    forall s1 s2,
-      ~ test s1 ->
-      Korder s2 s1 ->
-      loop_access_fin R test s1 (Terminating s2)
-| loop_access_Error:
-    forall s1 s2,
-      test s1 ->
-      Korder s2 s1 ->
-      R s2 Error ->
-      loop_access_fin R test s1 Error
-| loop_access_fin_NonTerminating:
-    forall s1 s2,
-      test s1 ->
-      Korder s2 s1 ->
-      R s2 NonTerminating ->
-      loop_access_fin R test s1 NonTerminating
-| loop_access_step:
-    forall s1 s2 s3 s4 ms,
-      test s1 ->
-      Korder s2 s1 ->
-      R s2 (Terminating s3) ->
-      Korder s4 s3 ->
-      loop_access_fin R test s4 ms ->
-      loop_access_fin R test s1 ms.
-
-Inductive loop_access_inf
-          {state: Type}
-          {kiM: KripkeIntuitionisticModel state}
-          (R: state -> MetaState state -> Prop)
-          (test: state -> Prop): state -> Prop :=
-| loop_access_inf_NonTerminating:
-    forall (s1 s2 s3: nat -> state),
-      (forall n, test (s1 n)) ->
-      (forall n, Korder (s2 n) (s1 n)) ->
-      (forall n, R (s2 n) (Terminating (s3 n))) ->
-      (forall n, Korder (s1 (S n)) (s3 n)) ->
-      loop_access_inf R test (s1 0).
-
-Inductive loop_access
-          {state: Type}
-          {kiM: KripkeIntuitionisticModel state}
-          (R: state -> MetaState state -> Prop)
-          (test: state -> Prop): state -> MetaState state -> Prop :=
-| loop_access_loop_access_fin:
-    forall s ms, loop_access_fin R test s ms ->
-      loop_access R test s ms
-| loop_access_loop_access_inf:
-    forall s, loop_access_inf R test s ->
-      loop_access R test s NonTerminating.
-
-Class ImpBigStepSemantics (P: ProgrammingLanguage) {iP: ImperativeProgrammingLanguage P} (state: Type) {kiM: KripkeIntuitionisticModel state} (BSS: BigStepSemantics P state): Type := {
-  eval_bool: state -> bool_expr -> Prop;
-  eval_bool_stable: forall b, Korder_stable (fun s => eval_bool s b);
-  access_Ssequence: forall c1 c2 s ms,
-    access s (Ssequence c1 c2) ms ->
-    exists ms' ms'',
-      access s c1 ms' /\ lift_Korder ms'' ms' /\ lift_access ms'' c2 ms;
-  access_Sifthenelse: forall b c1 c2 s ms,
-    access s (Sifthenelse b c1 c2) ms ->
-    (eval_bool s b /\ exists s', Korder s' s /\ access s' c1 ms) \/
-    (~ eval_bool s b /\ exists s', Korder s' s /\ access s' c2 ms);
-  access_Swhile: forall b c s ms,
-    access s (Swhile b c) ms ->
-    loop_access (fun s ms => access s c ms) (fun s => eval_bool s b) s ms
-}.
-
-Section soundness.
+Section partial_soundness.
 
 Existing Instance unit_kMD.
+Import Partial.
 
 Context {P: ProgrammingLanguage}
         {iP: ImperativeProgrammingLanguage P}
@@ -125,27 +54,6 @@ Proof.
     inversion H4; auto.
 Qed.
 
-Lemma hoare_seq_total_sound: forall c1 c2 P1 P2 P3,
-  triple_total_valid P1 c1 P2 ->
-  triple_total_valid P2 c2 P3 ->
-  triple_total_valid P1 (Ssequence c1 c2) P3.
-Proof.
-  intros.
-  unfold triple_total_valid in *.
-  intros s ms ? ?.
-  apply access_Ssequence in H2.
-  destruct H2 as [ms' [ms'' [? [? ?]]]].
-  specialize (H s ms' H1 H2).
-  destruct ms' as [| | s'].
-  + inversion H.
-  + inversion H.
-  + inversion H3; subst.
-    eapply sat_mono in H; [| exact H7].
-    clear H2 H7 H3 s'; rename x into s'.
-    apply (H0 s' ms); auto.
-    inversion H4; auto.
-Qed.
-
 Lemma hoare_if_partial_sound: forall b c1 c2 B P1 P2,
   (forall s, s |= B <-> eval_bool s b) ->
   triple_partial_valid (P1 && B) c1 P2 ->
@@ -156,7 +64,8 @@ Proof.
   unfold triple_partial_valid in *.
   intros s ms ? ?.
   apply access_Sifthenelse in H3.
-  destruct H3; destruct H3 as [? [s' [? ?]]].
+  destruct H3 as [| [[? [s' [? ?]]] | [? [s' [? ?]]]]].
+  + subst; auto.
   + assert (KRIPKE: s |= P1 && B) by (rewrite sat_andp; firstorder).
     eapply sat_mono in H6; [| eassumption].
     apply (H0 s'); auto.
@@ -169,34 +78,6 @@ Proof.
       pose proof eval_bool_stable b _ _ H6.
       simpl in H7, H8.
       rewrite H8 in H7; exfalso; auto.
-    } Unfocus.
-    eapply sat_mono in H6; [| eassumption].
-    apply (H1 s'); auto.
-Qed.
-
-Lemma hoare_if_total_sound: forall b c1 c2 B P1 P2,
-  (forall s, s |= B <-> eval_bool s b) ->
-  triple_total_valid (P1 && B) c1 P2 ->
-  triple_total_valid (P1 && ~~ B) c2 P2 ->
-  triple_total_valid P1 (Sifthenelse b c1 c2) P2.
-Proof.
-  intros.
-  unfold triple_total_valid in *.
-  intros s ms ? ?.
-  apply access_Sifthenelse in H3.
-  destruct H3; destruct H3 as [? [s' [? ?]]].
-  + assert (KRIPKE: s |= P1 && B) by (rewrite sat_andp; firstorder).
-    eapply sat_mono in H6; [| eassumption].
-    apply (H0 s'); auto.
-  + assert (KRIPKE: s |= P1 && ~~ B).
-    Focus 1. {
-      rewrite sat_andp; split; auto.
-      unfold negp; rewrite sat_impp.
-      intros.
-      rewrite H in H7.
-      pose proof eval_bool_stable b _ _ H6.
-      simpl in H7, H8.
-      tauto.
     } Unfocus.
     eapply sat_mono in H6; [| eassumption].
     apply (H1 s'); auto.
@@ -233,6 +114,73 @@ Proof.
     eapply sat_mono in H6; [| eassumption].
     eapply sat_mono; [eassumption |].
     exact (H0 _ _ H6 H4).
+Qed.
+
+End partial_soundness.
+
+Section total_soundness.
+
+Existing Instance unit_kMD.
+Import Total.
+
+Context {P: ProgrammingLanguage}
+        {iP: ImperativeProgrammingLanguage P}
+        {MD: Model}
+        {kiM: KripkeIntuitionisticModel model}
+        {BSS: BigStepSemantics P model}
+        {nBSS: NormalBigStepSemantics P model BSS}
+        {iBSS: ImpBigStepSemantics P model BSS}.
+
+Context {L: Language} {nL: NormalLanguage L} {pL: PropositionalLanguage L} {SL: SeparationLanguage L} {SM: Semantics L MD} {kiSM: KripkeIntuitionisticSemantics L MD tt SM}.
+
+
+Lemma hoare_seq_total_sound: forall c1 c2 P1 P2 P3,
+  triple_total_valid P1 c1 P2 ->
+  triple_total_valid P2 c2 P3 ->
+  triple_total_valid P1 (Ssequence c1 c2) P3.
+Proof.
+  intros.
+  unfold triple_total_valid in *.
+  intros s ms ? ?.
+  apply access_Ssequence in H2.
+  destruct H2 as [ms' [ms'' [? [? ?]]]].
+  specialize (H s ms' H1 H2).
+  destruct ms' as [| | s'].
+  + inversion H.
+  + inversion H.
+  + inversion H3; subst.
+    eapply sat_mono in H; [| exact H7].
+    clear H2 H7 H3 s'; rename x into s'.
+    apply (H0 s' ms); auto.
+    inversion H4; auto.
+Qed.
+
+Lemma hoare_if_total_sound: forall b c1 c2 B P1 P2,
+  (forall s, s |= B <-> eval_bool s b) ->
+  triple_total_valid (P1 && B) c1 P2 ->
+  triple_total_valid (P1 && ~~ B) c2 P2 ->
+  triple_total_valid P1 (Sifthenelse b c1 c2) P2.
+Proof.
+  intros.
+  unfold triple_total_valid in *.
+  intros s ms ? ?.
+  apply access_Sifthenelse in H3.
+  destruct H3; destruct H3 as [? [s' [? ?]]].
+  + assert (KRIPKE: s |= P1 && B) by (rewrite sat_andp; firstorder).
+    eapply sat_mono in H6; [| eassumption].
+    apply (H0 s'); auto.
+  + assert (KRIPKE: s |= P1 && ~~ B).
+    Focus 1. {
+      rewrite sat_andp; split; auto.
+      unfold negp; rewrite sat_impp.
+      intros.
+      rewrite H in H7.
+      pose proof eval_bool_stable b _ _ H6.
+      simpl in H7, H8.
+      tauto.
+    } Unfocus.
+    eapply sat_mono in H6; [| eassumption].
+    apply (H1 s'); auto.
 Qed.
 
 Lemma hoare_while_total_sound:
@@ -311,4 +259,4 @@ Proof.
   } Unfocus.
 Qed.
 
-End soundness.
+End total_soundness.
